More stuff in sheaves.

sheaves/shf.v
@@ -30,6 +30,18 @@ Axiom funext : forall A (B : A -> Type) (f g : forall x, B x),
   (forall x, f x = g x) -> f = g.
 Axiom pi : forall (A : Prop) (p q : A), p = q.
 
+Lemma sig_eq : forall {A} {P : A -> Prop} (p q : @sig A P), proj1_sig p = proj1_sig q -> p = q.
+Proof.
+intros A P [p hp] [q hq]; cbn.
+revert hq; destruct 1; f_equal; apply pi.
+Qed.
+
+Lemma sig_eq_rev : forall {A} {P : A -> Prop} (p q : @sig A P), p = q -> proj1_sig p = proj1_sig q.
+Proof.
+intros A P p q []; reflexivity.
+Qed.
+
+
 Lemma is_Sheaf_Sheaf' : forall J A, isSheaf' J A -> isSheaf J A.
 Proof.
 intros J A hA.
@@ -64,56 +76,346 @@ unshelve econstructor.
   intros p; rewrite (hf p); reflexivity.
 Defined.
 
-Lemma Prod_isSheaf' : forall (J : site) (A : Type) (B : A -> Type),
-  (forall x, isSheaf' J (B x)) -> isSheaf' J (forall x, B x).
-Proof.
-intros J A B Bε.
-unshelve econstructor.
-+ refine (fun P i f x => (Bε x).(shf_elt' _ _) P i (fun p => f p x)).
-+ intros P i f; cbn.
-  apply (Bε x).
-  intros p; rewrite (hf p); reflexivity.
-Defined.
-
-(** Sheafification *)
-
-Axiom Q : forall (J : site) (A : Type), Type.
-Axiom qc : forall {J : site} {A} (P : Prop), J P -> (P -> A) -> Q J A.
-Axiom q_eq : forall {J : site} {A : Type}
-  (P Q : Prop) (i : J P) (j : J Q) (φ : P -> A) (ψ : Q -> A) (α : P -> Q),
-  (forall p, φ p = ψ (α p)) ->
-  qc P i φ = qc Q j ψ.
-
-Axiom Q_rect : forall {J : site} {A}
-  (F : Q J A -> Type)
-  (u : forall P (i : J P) (φ : P -> A), F (qc P i φ))
-  (ue : forall P Q (i : J P) (j : J Q) (φ : P -> A) (ψ : Q -> A) (α : P -> Q)
-    (h : forall p, φ p = ψ (α p)),
-    match q_eq P Q i j φ ψ α h in _ = z return F z with eq_refl => u P i φ end = u Q j ψ ),
-  forall (q : Q J A), F q.
-
-Axiom Q_rect_qc : forall J A F u ue P i φ,
-  @Q_rect J A F u ue (qc P i φ) = u P i φ.
-
 Definition isSeparated (J : site) (A : Type) :=
   forall P (i : J P) (c : P -> A) (x y : A),
       (forall p : P, x = c p) -> (forall p : P, y = c p) -> x = y.
 
-Lemma isSeparated_Q : forall J (A : Type), isSeparated J (Q J A).
+Lemma closed_diag_isSeparated : forall (J : site) A,
+  isSeparated J A -> (forall x y : A, J (x = y) -> x = y).
 Proof.
-intros J A P i c.
-unshelve refine (Q_rect (fun x => forall y, (forall p : P, x = c p) -> (forall p : P, y = c p) -> x = y) _ _).
-+ intros P' j φ y hx; revert y.
-  unshelve refine (Q_rect _ _ _).
-  - intros P'' k ψ hy.
-    assert (e : forall p : P, qc P' j φ = qc P'' k ψ).
-    { intros p; rewrite (hx p), (hy p); reflexivity. }
-    apply e.
-    apply funext in hx; apply funext in hy.
-    rewrite <- hx in hy.
-    admit.
-  -
-Abort.
+intros J A hA x y e.
+unshelve refine (hA (x = y) e (fun _ => y) x y (fun e => e) (fun _ => eq_refl)).
+Defined.
+
+Lemma isSeparated_closed_diag : forall (J : site) A,
+  (forall x y : A, J (x = y) -> x = y) -> isSeparated J A.
+Proof.
+intros J A hA P i c x y hx hy.
+refine (hA _ _ _).
+refine (@ste_mon J _ _ i _).
+intros p; apply ste_top.
+rewrite (hx p), (hy p); reflexivity.
+Defined.
+
+Definition PropJ (J : site) := {P : Prop | J P -> P}.
+
+Definition liftJ (J : site) (P : Prop) : PropJ J.
+Proof.
+exists (J P).
+refine (fun p => ste_mon _ _ p (fun p => p)).
+Defined.
+
+(** Sheafification à la MacLane-Moerdijk *)
+
+Definition Sh (J : site) (A : Type) :=
+  { P : A -> PropJ J | J (exists x : A, forall y, proj1_sig (P y) <-> J (x = y)) }.
+
+Definition Sh_η (J : site) (A : Type) (x : A) : Sh J A.
+Proof.
+exists (fun y => liftJ J (x = y)).
+apply ste_top; exists x; tauto.
+Defined.
+
+Definition Sh_bind (J : site) (A B : Type) (m : Sh J A) (f : A -> Sh J B) : Sh J B.
+Proof.
+destruct m as [P hP].
+unshelve econstructor.
++ refine (fun y => liftJ J (exists x : A, proj1_sig (P x) /\ proj1_sig (proj1_sig (f x) y))).
++ refine (ste_mon _ _ hP _); clear hP; intros hP.
+  destruct hP as [x hx].
+  remember (f x) as Q.
+  destruct Q as [Q HQ]; cbn in *.
+  refine (ste_mon _ _ HQ _); intros HQ'.
+  replace HQ with (@ste_top J _ HQ') in HeqQ by apply pi.
+  clear HQ; destruct HQ' as [y hy].
+  apply sig_eq_rev in HeqQ; cbn in HeqQ; subst Q.
+  apply ste_top; exists y; intros y'; split; intro H.
+  - refine (ste_mon _ _ H _); clear H; intros [x' [Hl Hr]].
+    assert (e : J (x = x')).
+    { apply hx; assumption. }
+    refine (ste_mon _ _ e _); clear e; intros e; subst x'.
+    apply hy; assumption.
+  - refine (ste_mon _ _ H _); clear H; intros H; subst y'.
+    apply ste_top; exists x; split.
+    { apply hx, ste_top; reflexivity. }
+    { apply hy, ste_top; reflexivity. }
+Defined.
+
+Lemma isSheaf_subobj (J : site) (A : Type) (P : A -> Prop)
+  (hA : isSheaf J A) (hP : forall x, J (P x) -> P x) : isSheaf J {x : A | P x}.
+Proof.
+apply is_Sheaf_Sheaf'.
+apply is_Sheaf'_Sheaf in hA.
+unshelve econstructor.
++ intros Q j x.
+  unshelve econstructor.
+  - refine (hA.(shf_elt' _ _) Q j (fun q => proj1_sig (x q))).
+  - apply hP.
+    unshelve refine (@ste_mon J _ _ j _).
+    intro j'; apply ste_top.
+    replace (fun q => proj1_sig (x q)) with (fun _ : Q => proj1_sig (x j')).
+    2: { apply funext; intros j''; repeat f_equal; apply pi. }
+    rewrite <- (shf_spc' J A hA Q j).
+    destruct (x j'); cbn; assumption.
++ intros Q j [x hx]; cbn.
+  match goal with [ |- _ = exist ?P ?x ?p ] => generalize p as hx' end.
+  rewrite <- shf_spc'; intros; f_equal; apply pi.
+Defined.
+
+Axiom propext : forall (A B : Prop), (A <-> B) -> A = B.
+
+Lemma isSeparated_Sh : forall J A, isSeparated J (Sh J A).
+Proof.
+intros J A; apply isSeparated_closed_diag. intros [P HP] [Q HQ] H; cbn.
+apply sig_eq; cbn.
+apply funext; intros z. apply sig_eq; apply propext.
+match goal with [ |- ?P ] => cut (J P) end.
++ clear; intros H; split; intros H';
+  match goal with [ |- proj1_sig ?P ] => apply (proj2_sig P) end;
+  refine (ste_mon _ _ H _); intros []; apply ste_top; tauto.
++ refine (ste_mon _ _ H _); clear H; intros H.
+  apply sig_eq_rev in H; cbn in H.
+  rewrite H; apply ste_top; tauto.
+Defined.
+
+Lemma PropJ_isSheaf (J : site) : isSheaf J (PropJ J).
+Proof.
+apply is_Sheaf_Sheaf'; unshelve econstructor.
++ intros P i f.
+  unshelve econstructor.
+  { refine (forall p : P, proj1_sig (f p)). }
+  { intros j p.
+    remember (f p) as Q; destruct Q as [Q HQ]; cbn in *.
+    apply HQ.
+    refine (ste_mon _ _ j _).
+    intros g.
+    specialize (g p).
+    rewrite <- HeqQ in g; cbn in g.
+    apply ste_top; assumption.
+  }
++ intros P i [Q HQ]; cbn.
+  apply sig_eq; cbn.
+  apply propext; split; [tauto|].
+  intros f. apply HQ.
+  refine (ste_mon _ _ i _).
+  intros p; apply ste_top; tauto.
+Defined.
+
+Lemma isSheaf_Sh : forall J A, isSeparated J A -> isSheaf J (Sh J A).
+Proof.
+intros J A HA.
+apply isSheaf_subobj.
++ apply Prod_isSheaf; intros; apply PropJ_isSheaf.
++ intros P HP.
+  refine (ste_mon _ _ HP (fun x => x)).
+Defined.
+
+Lemma Sh_bind_η : forall J A (x : Sh J A), Sh_bind J A _ x (Sh_η J A) = x.
+Proof.
+intros J A [P HP].
+apply sig_eq; cbn.
+apply funext; intros x; cbn.
+apply sig_eq; cbn; apply propext.
+split; intros H.
++ apply (proj2_sig (P x)).
+  refine (ste_mon _ _ H _); clear H; intros [y [Hy e]].
+  refine (ste_mon _ _ e _); clear e; intros ->; apply ste_top; assumption.
++ apply ste_top; exists x; split.
+  - assumption.
+  - apply ste_top; reflexivity.
+Qed.
+
+Lemma Sh_η_bind : forall J A B (x : A) f, Sh_bind J A B (Sh_η J A x) f = f x.
+Proof.
+intros J A B x f; apply sig_eq; cbn.
+apply funext; intros y; cbn; apply sig_eq; cbn; apply propext; split; intros H.
++ apply (proj2_sig (proj1_sig (f x) y)).
+  refine (ste_mon _ _ H _); clear H; intros [x' [e Hx]].
+  refine (ste_mon _ _ e _); clear e; intros e; subst x'.
+  apply ste_top; assumption.
++ apply ste_top; exists x; split.
+  - apply ste_top; reflexivity.
+  - assumption.
+Qed.
+
+Lemma Sh_bind_bind : forall J A B C (x : Sh J A) f g,
+  Sh_bind J B C (Sh_bind J A B x f) g = Sh_bind J A C x (fun x => Sh_bind J B C (f x) g).
+Proof.
+intros J A B C [P HP] f g; apply sig_eq; cbn.
+apply funext; intros z; apply sig_eq; cbn; apply propext; cbn; split; intros H.
++ refine (ste_mon _ _ H _); clear H; intros [y [hy hg]].
+  refine (ste_mon _ _ hy _); clear hy; intros [x [hx hf]].
+  apply ste_top; exists x; split; [assumption|].
+  remember (f x) as Q; destruct Q as [Q HQ]; cbn.
+  apply sig_eq_rev in HeqQ; cbn in HeqQ; subst Q; cbn in *.
+  apply ste_top; exists y; split; [assumption|].
+  assumption.
++ refine (ste_mon _ _ H _); clear H; intros [x [hx hf]].
+  remember (f x) as Q; destruct Q as [Q HQ]; cbn.
+  apply sig_eq_rev in HeqQ; cbn in HeqQ; subst Q; cbn in *.
+  refine (ste_mon _ _ hf _); clear hf; intros [y [hy hz]].
+  apply ste_top; exists y; split; [|assumption].
+  apply ste_top; exists x; split; assumption.
+Qed.
+
+Lemma Sh_idempotent : forall J A (x : Sh J A),
+  Sh_η J (Sh J A) x = Sh_bind J A (Sh J A) x (fun x => Sh_η J (Sh J A) (Sh_η J A x)).
+Proof.
+intros J A [P HP]; cbn; apply sig_eq; cbn.
+apply funext; intros [Q HQ]; apply sig_eq; cbn.
+apply propext; cbn; split; intros H.
++ refine (ste_mon _ _ H _); clear H; intros H.
+  apply sig_eq_rev in H; cbn in H.
+  subst Q; replace HQ with HP by apply pi; clear HQ.
+  refine (ste_mon _ _ HP _); intros HP'.
+  replace HP with (@ste_top J _ HP') by apply pi; clear HP; rename HP' into HP.
+  destruct HP as [x Hx]; apply ste_top; exists x.
+  split; [now apply Hx, ste_top, eq_refl|].
+  apply ste_top; apply sig_eq; cbn.
+  apply funext; intros x'; apply sig_eq, propext; cbn; split;
+  intros; apply Hx; assumption.
++ cut (J (P = Q)).
+  { clear H; intros H.
+    refine (ste_mon _ _ H _); clear H; intros H.
+    revert HP HQ; destruct H; intros HP HQ.
+    replace HP with HQ by apply pi; apply ste_top; reflexivity. }
+  refine (ste_mon _ _ H _); clear H; intros [x [Hx H]].
+  refine (ste_mon _ _ H _); clear H; intros H; apply sig_eq_rev in H; cbn in H.
+  rewrite <- H; clear Q HQ H.
+  refine (ste_mon _ _ HP _); clear HP; intros [x' HP].
+  assert (e : J (x' = x)).
+  { apply HP; assumption. }
+  refine (ste_mon _ _ e _); clear e; intro e; subst x'.
+  apply ste_top; apply funext; intros x'; apply sig_eq; apply propext; split; intros H; cbn in *.
+  - apply HP; assumption.
+  - apply HP; assumption.
+Qed.
+
+(** Sheafification with quotients *)
+
+Axiom Quo : forall (A : Type) (R : A -> A -> Prop), Type.
+Axiom quo : forall {A} R (x : A), Quo A R.
+Axiom quo_eq : forall {A} {R : A -> A -> Prop} (x y : A) (e : R x y), quo R x = quo R y.
+
+Axiom quo_rect : forall {A} {R : A -> A -> Prop} (P : Quo A R -> Type)
+    (u : forall x : A, P (quo R x))
+    (uε : forall (x y : A) (r : R x y), match quo_eq x y r in _ = z return P z with eq_refl => u x end = u y),
+    forall q : Quo A R, P q.
+
+Axiom quo_rect_eq : forall A R P u uε (x : A), @quo_rect A R P u uε (quo R x) = u x.
+
+Definition quo_elim : forall {A} {R : A -> A -> Prop} (P : Type)
+    (u : A -> P)
+    (uε : forall (x y : A) (r : R x y), u x = u y),
+    forall q : Quo A R, P.
+Proof.
+refine (fun A R P u uε => @quo_rect A R (fun _ => P) u _).
+{ intros x y r; destruct (@quo_eq A R x y r); apply uε, r. }
+Defined.
+
+Lemma quo_elim_eq : forall A R P u uε (x : A), @quo_elim A R P u uε (quo R x) = u x.
+Proof.
+intros; unfold quo_elim.
+refine (quo_rect_eq _ _ _ _ _ _).
+Qed.
+
+Inductive clos {A} (R : A -> A -> Prop) : A -> A -> Prop :=
+| clos_incl : forall x y, R x y -> clos R x y
+| clos_refl : forall x, clos R x x
+| clos_trns : forall x y z, clos R x y -> clos R y z -> clos R x z
+| clos_symm : forall x y, clos R x y -> clos R y x.
+
+(** We need propext to prove this from the other quotient axioms??? *)
+Axiom quo_inv : forall {A} {R : A -> A -> Prop} (x y : A) (e : quo R x = quo R y), clos R x y.
+
+
+Record T (J : site) (A : Type) := {
+  t_prp : Prop;
+  t_prf : J t_prp;
+  t_elt : (t_prp -> A);
+}.
+
+Arguments t_prp {_ _}.
+Arguments t_prf {_ _}.
+Arguments t_elt {_ _}.
+
+Definition Tr {J A} (x y : T J A) : Prop :=
+  exists (α : x.(t_prp) -> y.(t_prp)), forall (p : x.(t_prp)), x.(t_elt) p = y.(t_elt) (α p).
+
+Definition ShQ J A := Quo (T J A) Tr.
+
+(*
+Lemma Tr_eq : forall (J : site) (A : Type) (pX pY : T J A)
+  (p : t_prp pX) (q : t_prp pY), clos Tr pY pX -> t_elt pX p = t_elt pY q.
+Proof.
+induction 1.
++ destruct H as [α e].
+  symmetry; replace p with (α q) by apply pi.
+  apply e.
++ replace p with q by apply pi; reflexivity.
++ transitivity.
+  - apply IHclos2.
+  - apply IHclos1.
++ symmetry; apply IHclos.
+Qed.
+*)
+
+Lemma Tr_eq : forall (J : site) (A : Type) (P : Prop) (i : J P) 
+  (x : P -> A) (Q : Prop) (j : J Q) (y : Q -> A),
+  quo Tr {| t_prp := Q; t_prf := j; t_elt := y |} =
+  quo Tr {| t_prp := P; t_prf := i; t_elt := x |} ->
+  forall (p : P) (q : Q), x p = y q.
+Proof.
+Admitted.
+
+Lemma isSeparated_Q : forall J (A : Type), isSeparated J (ShQ J A).
+Proof.
+intros J A R k c x y hx hy.
+revert x hx y hy; unshelve refine (quo_rect _ (fun x hx => quo_rect _ (fun y hy => _) _) _).
++ destruct x as [P i x].
+  destruct y as [Q j y].
+  unshelve refine (let z : T J A := Build_T J A (R /\ P /\ Q) _ _ in _).
+  { refine (ste_mon _ _ i (fun i => ste_mon _ _ j (fun j => ste_mon _ _ k (fun k => ste_top _ (conj k (conj i j)))))). }
+  { intros [_ [p _]]; refine (x p). }
+  transitivity (quo Tr z); [symmetry|]; apply quo_eq.
+  - unshelve econstructor; cbn.
+    { intros [_ [p _]]; exact p. }
+    { intros [_ [p _]]; reflexivity. }
+  - unshelve econstructor; cbn.
+    { intros [_ [_ q]]; exact q. }
+    { intros [r [p q]].
+      clear z.
+      specialize (hx r).
+      specialize (hy r).
+      rewrite <- hx in hy; clear hx.
+      eapply Tr_eq, hy.
+    }
++ intros; apply pi.
++ intros; apply pi.
+Defined.
+
+Lemma isSheaf_ShQ : forall J (A : Type), isSeparated J A -> isSheaf J (ShQ J A).
+Proof.
+intros J A hA.
+
+unshelve econstructor.
++ intros P i x.
+  refine (quo _ _); unshelve econstructor.
+  - refine (exists p : P, _).
+(*
+    unshelve refine (quo_elim Prop _ _ (x p)).
+    { intros [Q _ _]; exact (P /\ Q). }
+    { clear - hA; intros [Q j y] [R k z].
+      intros [α f]; cbn in *.
+cbn.
+*)
+  exact True.
+  - admit.
+  - intros r.
+    unshelve refine (quo_elim _ _ _ (x _)).
+    
+intros [p q].
+
 
 Definition bind {J A B} : Q J A -> (A -> Q J B) -> Q J B.
 Proof.
